case_study/RiscvPmp/Contracts.v
@@ -1239,6 +1239,13 @@ Module Import RiscvPmpSpecification <: Specification RiscvPmpBase RiscvPmpProgra
                asn_pmp_addr_access (term_var "entries") (term_var p)
           |}.
 
+        Definition lemma_close_mmio_write (immm : Bitvector.bv.bv 12) (r1 r2 : Reg ty_xlenbits) (widthh : WordWidth): SepLemma (close_mmio_write immm r1 r2 widthh) :=
+          {| lemma_logic_variables := [];
+             lemma_patterns        := [env];
+             lemma_precondition    := ⊤;
+             lemma_postcondition   := ⊤;
+          |}.
+
         Definition LEnv : LemmaEnv :=
           fun Δ l =>
             match l with
@@ -1250,6 +1257,7 @@ Module Import RiscvPmpSpecification <: Specification RiscvPmpBase RiscvPmpProgra
             | close_ptsto_instr       => lemma_close_ptsto_instr
             | extract_pmp_ptsto bytes => lemma_extract_pmp_ptsto bytes
             | return_pmp_ptsto bytes  => lemma_return_pmp_ptsto bytes
+            | close_mmio_write immm r1 r2 widthh => lemma_close_mmio_write immm r1 r2 widthh
             end.
 
       End LemDef.
